\documentclass{article}
\usepackage{fullpage}

\newcommand{\U}{\,\mbox{\sf{U}}\,}
\newcommand{\A}{\mbox{\sf{A}}}
\newcommand{\E}{\mbox{\sf{E}}}
\newcommand{\AX}{\mbox{\sf{AX}}}
\newcommand{\EX}{\mbox{\sf{EX}}}
\newcommand{\AF}{\mbox{\sf{AF}}}
\newcommand{\EF}{\mbox{\sf{EF}}}
\newcommand{\AG}{\mbox{\sf{AG}}}
\newcommand{\EG}{\mbox{\sf{EG}}}

\newcommand{\mita}[1]{\mbox{\it{{#1}}}}
\newcommand{\mtt}[1]{\mbox{\tt{{#1}}}}
\newcommand{\msf}[1]{\mbox{\sf{{#1}}}}
\newcommand{\mrm}[1]{\mbox{\rm{{#1}}}}
\newcommand{\mth}[1]{\({#1}\)}

\newcommand{\ttlb}{\mbox{\tt \char'173}}
\newcommand{\ttrb}{\mbox{\tt \char'175}}

\begin{document}

\begin{quote}\begin{verbatim}

@@
@@

f();
...
?g();
...
h();
\end{verbatim}\end{quote}

\[\begin{array}{l}
\mita{\sf{let}} \, \mita{\_aftret} = \msf{After} \vee \msf{Return} \, \mita{\sf{in}} \, \mita{f();} \wedge (\AX(\mita{\sf{let}} \, \mita{l4} = (\mita{g();} \wedge (\AX(\mita{\sf{let}} \, \mita{l2} = \mita{h();}\\\mbox{} \, \mita{\sf{in}} \, (\mita{\sf{let}} \, \mita{l3} = \neg (\mita{h();} \vee \mita{g();}) \, \mita{\sf{in}} \, (\A[\mita{l3} \U (\mita{l2} \vee \mita{\_aftret})]
) \wedge (\E[\mita{l3} \U \mita{l2}]
)
)
)))\\\mbox{} \vee (\mita{\sf{let}} \, \mita{l0} = \mita{h();} \, \mita{\sf{in}} \, (\mita{\sf{let}} \, \mita{l1} = \neg (\mita{g();} \vee \mita{h();}) \, \mita{\sf{in}} \, (\A[\mita{l1} \U (\mita{l0} \vee \mita{\_aftret})]
) \wedge (\E[\mita{l1}\\\mbox{} \U \mita{l0}]
)
)
) \, \mita{\sf{in}} \, (\mita{\sf{let}} \, \mita{l5} = \neg (\mita{g();} \vee \mita{f();}) \, \mita{\sf{in}} \, (\A[\mita{l5} \U (\mita{l4} \vee \mita{\_aftret})]
) \wedge (\E[\mita{l5}\\\mbox{} \U \mita{l4}]
)
)
))

\end{array}\]

\begin{quote}\begin{verbatim}

@@
@@

foo(...) {
  
(
  -f-(-3-, -E-)-;
    >>> f(3, 3, E);
  
|
  -f-(-E-, -4-)-;
    >>> f(E, 4, 4);
  
|
  -E-;
    >>> g(E);
  
)
  
(
  -f-(-3-, -X-)-;
    >>> f(3, 3, X);
  
|
  -f-(-Y-, -4-)-;
    >>> f(Y, 4, 4);
  
|
  -Z-;
    >>> g(Z);
  
)
  
(
  -f-(-3-)-;
    >>> f(3, 3);
  
|
  -f-(-4-)-;
    >>> f(4, 4);
  
)
}
\end{verbatim}\end{quote}

\[\begin{array}{l}
(\exists \mita{foo} . \mita{foo(...) }) \wedge (\AX(\exists \mita{v1} . (\mita{{\ttlb}
  } \wedge \msf{Paren}(v1) \wedge (\AX(\mita{\sf{let}} \, \mita{l4} = (\mita{\sf{let}} \, \mita{l1} = (\mita{\sf{let}} \, \mita{l0} = \mita{
{\ttrb}}\\\mbox{} \wedge \msf{Paren}(v1) \, \mita{\sf{in}} \, ((\exists \mita{v5} . \mita{-f-(-3-)-;
  \mth{>}\mth{>}\mth{>} f(3, 3);}_{\mita{v5}}) \wedge (\AX\mita{l0})) \vee ((\exists \mita{v4} . \mita{-f-(-4-)-;
  \mth{>}\mth{>}\mth{>} f(4, 4);}_{\mita{v4}})\\\mbox{} \wedge (\AX\mita{l0}))
) \, \mita{\sf{in}} \, (\mita{\sf{let}} \, \mita{l3} = \exists \mita{X} . \exists \mita{v10} . \mita{-f-(-3-, -X-)-;
  \mth{>}\mth{>}\mth{>} f(3, 3, X);}_{\mita{v10}}\\\mbox{} \, \mita{\sf{in}} \, (\exists \mita{X} . ((\exists \mita{v9} . \mita{-f-(-3-, -X-)-;
  \mth{>}\mth{>}\mth{>} f(3, 3, X);}_{\mita{v9}}) \wedge (\AX\mita{l1}))) \vee (\mita{\sf{let}} \, \mita{l2} = \exists \mita{Y}\\\mbox{} . \exists \mita{v8} . \mita{-f-(-Y-, -4-)-;
  \mth{>}\mth{>}\mth{>} f(Y, 4, 4);}_{\mita{v8}} \, \mita{\sf{in}} \, ((\neg \mita{l3}) \wedge (\exists \mita{Y} . ((\exists \mita{v7} . \mita{-f-(-Y-, -4-)-;
  \mth{>}\mth{>}\mth{>} f(Y, 4, 4);}_{\mita{v7}})\\\mbox{} \wedge (\AX\mita{l1})))) \vee ((\neg \mita{l2}) \wedge (\neg \mita{l3}) \wedge (\exists \mita{Z} . ((\exists \mita{v6} . \mita{-Z-;
  \mth{>}\mth{>}\mth{>} g(Z);}_{\mita{v6}}) \wedge (\AX\mita{l1}))))\\\mbox{}
)
)
) \, \mita{\sf{in}} \, (\mita{\sf{let}} \, \mita{l6} = \exists \mita{E} . \exists \mita{v15} . \mita{-f-(-3-, -E-)-;
  \mth{>}\mth{>}\mth{>} f(3, 3, E);}_{\mita{v15}} \, \mita{\sf{in}} \, (\exists \mita{E}\\\mbox{} . ((\exists \mita{v14} . \mita{-f-(-3-, -E-)-;
  \mth{>}\mth{>}\mth{>} f(3, 3, E);}_{\mita{v14}}) \wedge (\AX\mita{l4}))) \vee (\mita{\sf{let}} \, \mita{l5} = \exists \mita{E}\\\mbox{} . \exists \mita{v13} . \mita{-f-(-E-, -4-)-;
  \mth{>}\mth{>}\mth{>} f(E, 4, 4);}_{\mita{v13}} \, \mita{\sf{in}} \, ((\neg \mita{l6}) \wedge (\exists \mita{E} . ((\exists \mita{v12} . \mita{-f-(-E-, -4-)-;
  \mth{>}\mth{>}\mth{>} f(E, 4, 4);}_{\mita{v12}})\\\mbox{} \wedge (\AX\mita{l4})))) \vee ((\neg \mita{l5}) \wedge (\neg \mita{l6}) \wedge (\exists \mita{E} . ((\exists \mita{v11} . \mita{-E-;
  \mth{>}\mth{>}\mth{>} g(E);}_{\mita{v11}}) \wedge (\AX\mita{l4}))))\\\mbox{}
)
)
)))))
\end{array}\]

\begin{quote}\begin{verbatim}

@@
@@

p(
    <<< int hostptr, 
  char buffer) {
  -int -hostptr-;
}
\end{verbatim}\end{quote}

\[\begin{array}{l}
\exists \mita{hostptr} . ((\exists \mita{buffer} . \exists \mita{v0} . \mita{p(
    <<< int hostptr, 
  char buffer) }_{\mita{v0}})\\\mbox{} \wedge (\AX(\exists \mita{v1} . (\mita{{\ttlb}
  } \wedge \msf{Paren}(v1) \wedge (\AX((\exists \mita{v4} . \mita{-int -hostptr-;}_{\mita{v4}}) \wedge (\AX(\mita{
{\ttrb}} \wedge \msf{Paren}(v1)))))))))
\end{array}\]

\begin{quote}\begin{verbatim}

@@
@@

f(X);
-...   WHEN != -h-(-X-)
g(Y);
\end{verbatim}\end{quote}

\[\begin{array}{l}
\mita{\sf{let}} \, \mita{\_aftret} = \msf{After} \vee \msf{Return} \, \mita{\sf{in}} \, \exists \mita{X} . (\mita{f(X);} \wedge (\AX(\mita{\sf{let}} \, \mita{l0} = \exists \mita{Y} . \mita{g(Y);} \, \mita{\sf{in}} \, (\mita{\sf{let}} \, \mita{l1} = (\exists \mita{v1}\\\mbox{} . \mita{-\_S0}_{\mita{v1}}) \wedge (\neg (\exists \mita{v4} . \mita{-h-(-X-)}_{\mita{v4}})) \wedge (\neg ((\exists \mita{Y} . \mita{g(Y);}) \vee \mita{f(X);})) \, \mita{\sf{in}} \, (\A[\mita{l1} \U (\mita{l0}\\\mbox{} \vee \mita{\_aftret})]
) \wedge (\E[\mita{l1} \U \mita{l0}]
)
)
)))

\end{array}\]

\begin{quote}\begin{verbatim}

@@
@@

f(X);
-...
g(Y);
\end{verbatim}\end{quote}

\[\begin{array}{l}
\mita{\sf{let}} \, \mita{\_aftret} = \msf{After} \vee \msf{Return} \, \mita{\sf{in}} \, (\exists \mita{X} . \mita{f(X);}) \wedge (\AX(\mita{\sf{let}} \, \mita{l0} = \exists \mita{Y} . \mita{g(Y);} \, \mita{\sf{in}} \, (\mita{\sf{let}} \, \mita{l1} = (\exists \mita{v1}\\\mbox{} . \mita{-\_S0}_{\mita{v1}}) \wedge (\neg ((\exists \mita{Y} . \mita{g(Y);}) \vee (\exists \mita{X} . \mita{f(X);}))) \, \mita{\sf{in}} \, (\A[\mita{l1} \U (\mita{l0} \vee \mita{\_aftret})]
) \wedge (\E[\mita{l1}\\\mbox{} \U \mita{l0}]
)
)
))

\end{array}\]

\begin{quote}\begin{verbatim}

@@
@@

f(X);
g(Y);
h(X);
f(Y);
g(X);
h(Y);
\end{verbatim}\end{quote}

\[\begin{array}{l}
\exists \mita{X} . (\mita{f(X);} \wedge (\AX(\exists \mita{Y} . (\mita{g(Y);} \wedge (\AX(\mita{h(X);} \wedge (\AX(\mita{f(Y);} \wedge (\AX(\mita{g(X);} \wedge (\AX(\mita{h(Y);}))))))))))))
\end{array}\]

\begin{quote}\begin{verbatim}

@@
@@

f(X);
...
g(X);
h(X);
\end{verbatim}\end{quote}

\[\begin{array}{l}
\mita{\sf{let}} \, \mita{\_aftret} = \msf{After} \vee \msf{Return} \, \mita{\sf{in}} \, \exists \mita{X} . (\mita{f(X);} \wedge (\AX(\mita{\sf{let}} \, \mita{l0} = \mita{g(X);} \wedge (\AX(\mita{h(X);}))\\\mbox{} \, \mita{\sf{in}} \, (\mita{\sf{let}} \, \mita{l1} = \neg (\mita{g(X);} \vee \mita{f(X);}) \, \mita{\sf{in}} \, (\A[\mita{l1} \U (\mita{l0} \vee \mita{\_aftret})]
) \wedge (\E[\mita{l1} \U \mita{l0}]
)\\\mbox{}
)
)))

\end{array}\]

\begin{quote}\begin{verbatim}

@@
@@

if (X) {
  ...
} else {
  ...
}
f(X);
\end{verbatim}\end{quote}

\[\begin{array}{l}
\mita{\sf{let}} \, \mita{\_aftret} = \msf{After} \vee \msf{Return} \, \mita{\sf{in}} \, \exists \mita{X} . (\mita{if (X) } \wedge (\AX((\msf{TrueBranch} \rightarrow (\AX(\exists \mita{v2} . (\mita{{\ttlb}
  }\\\mbox{} \wedge \msf{Paren}(v2) \wedge (\AX(\mita{\sf{let}} \, \mita{l0} = \mita{
{\ttrb}} \wedge \msf{Paren}(v2) \, \mita{\sf{in}} \, (\AF(\mita{l0} \vee \mita{\_aftret})) \wedge (\EF\mita{l0})
))))))\\\mbox{} \wedge (\msf{FalseBranch} \rightarrow (\AX(\exists \mita{v5} . (\mita{{\ttlb}
  } \wedge \msf{Paren}(v5) \wedge (\AX(\mita{\sf{let}} \, \mita{l1} = \mita{
{\ttrb}} \wedge \msf{Paren}(v5) \, \mita{\sf{in}} \, (\AF(\mita{l1}\\\mbox{} \vee \mita{\_aftret})) \wedge (\EF\mita{l1})
)))))) \wedge (\msf{After} \rightarrow (\AX(\mita{f(X);}))))) \wedge (\EX(\msf{FalseBranch}))\\\mbox{} \wedge (\EX(\msf{After})))

\end{array}\]

\begin{quote}\begin{verbatim}

@@
@@

if (X) {
  ...
}
f(X);
\end{verbatim}\end{quote}

\[\begin{array}{l}
\mita{\sf{let}} \, \mita{\_aftret} = \msf{After} \vee \msf{Return} \, \mita{\sf{in}} \, \exists \mita{X} . (\mita{if (X) } \wedge (\AX((\msf{TrueBranch} \vee \msf{After}) \wedge (\msf{TrueBranch}\\\mbox{} \rightarrow (\AX(\exists \mita{v2} . (\mita{{\ttlb}
  } \wedge \msf{Paren}(v2) \wedge (\AX(\mita{\sf{let}} \, \mita{l0} = \mita{
{\ttrb}} \wedge \msf{Paren}(v2) \, \mita{\sf{in}} \, (\AF(\mita{l0} \vee \mita{\_aftret}))\\\mbox{} \wedge (\EF\mita{l0})
)))))) \wedge (\msf{After} \rightarrow (\AX(\mita{f(X);}))))) \wedge (\EX(\msf{After})))

\end{array}\]

\begin{quote}\begin{verbatim}

@@
@@

while (X) {
  ...
}
f(X);
\end{verbatim}\end{quote}

\[\begin{array}{l}
\mita{\sf{let}} \, \mita{\_aftret} = \msf{After} \vee \msf{Return} \, \mita{\sf{in}} \, \exists \mita{X} . (\mita{while (X) } \wedge (\AX((\msf{TrueBranch} \rightarrow (\AX(\exists \mita{v2}\\\mbox{} . (\mita{{\ttlb}
  } \wedge \msf{Paren}(v2) \wedge (\AX(\mita{\sf{let}} \, \mita{l0} = \mita{
{\ttrb}} \wedge \msf{Paren}(v2) \, \mita{\sf{in}} \, (\AF(\mita{l0} \vee \mita{\_aftret})) \wedge (\EF\mita{l0})\\\mbox{}
)))))) \wedge (\msf{After} \rightarrow (\AX(\mita{f(X);}))))) \wedge (\EX(\msf{After})))

\end{array}\]

\begin{quote}\begin{verbatim}

@@
@@

while (X) {
  ...
}
\end{verbatim}\end{quote}

\[\begin{array}{l}
\mita{\sf{let}} \, \mita{\_aftret} = \msf{After} \vee \msf{Return} \, \mita{\sf{in}} \, \exists \mita{X} . (\mita{while (X) } \wedge (\AX(\msf{TrueBranch} \rightarrow (\AX(\exists \mita{v1}\\\mbox{} . (\mita{{\ttlb}
  } \wedge \msf{Paren}(v1) \wedge (\AX(\mita{\sf{let}} \, \mita{l0} = \mita{
{\ttrb}} \wedge \msf{Paren}(v1) \, \mita{\sf{in}} \, (\AF(\mita{l0} \vee \mita{\_aftret})) \wedge (\EF\mita{l0})\\\mbox{}
))))))))

\end{array}\]

\begin{quote}\begin{verbatim}

@@
@@

{
  ...   WHEN != g(Y)
  f(X);
  ...   WHEN != h(Y)
}
\end{verbatim}\end{quote}

\[\begin{array}{l}
\mita{\sf{let}} \, \mita{\_aftret} = \msf{After} \vee \msf{Return} \, \mita{\sf{in}} \, \exists \mita{Y} . \exists \mita{X} . \exists \mita{v0} . (\mita{{\ttlb}
  } \wedge \msf{Paren}(v0) \wedge (\AX(\mita{\sf{let}} \, \mita{l2} = \mita{f(X);}\\\mbox{} \wedge (\AX(\mita{\sf{let}} \, \mita{l0} = \mita{
{\ttrb}} \wedge \msf{Paren}(v0) \, \mita{\sf{in}} \, (\mita{\sf{let}} \, \mita{l1} = (\neg \mita{h(Y)}) \wedge (\neg \mita{f(X);}) \, \mita{\sf{in}} \, (\A[\mita{l1} \U (\mita{l0}\\\mbox{} \vee \mita{\_aftret})]
) \wedge (\E[\mita{l1} \U \mita{l0}]
)
)
)) \, \mita{\sf{in}} \, (\mita{\sf{let}} \, \mita{l3} = (\neg \mita{g(Y)}) \wedge (\neg \mita{f(X);}) \, \mita{\sf{in}} \, (\A[\mita{l3} \U (\mita{l2}\\\mbox{} \vee \mita{\_aftret})]
) \wedge (\E[\mita{l3} \U \mita{l2}]
)
)
)))

\end{array}\]

\begin{quote}\begin{verbatim}

@@
@@

f(X);
...
-g-(-Y-)-;
  >>> h(X, Y);

\end{verbatim}\end{quote}

\[\begin{array}{l}
\mita{\sf{let}} \, \mita{\_aftret} = \msf{After} \vee \msf{Return} \, \mita{\sf{in}} \, \exists \mita{X} . (\mita{f(X);} \wedge (\AX(\mita{\sf{let}} \, \mita{l0} = \exists \mita{Y} . \exists \mita{v0} . \mita{-g-(-Y-)-;
  \mth{>}\mth{>}\mth{>} h(X, Y);}_{\mita{v0}}\\\mbox{} \, \mita{\sf{in}} \, (\mita{\sf{let}} \, \mita{l1} = \neg ((\exists \mita{Y} . \exists \mita{v2} . \mita{-g-(-Y-)-;
  \mth{>}\mth{>}\mth{>} h(X, Y);}_{\mita{v2}}) \vee \mita{f(X);}) \, \mita{\sf{in}} \, (\A[\mita{l1}\\\mbox{} \U (\mita{l0} \vee \mita{\_aftret})]
) \wedge (\E[\mita{l1} \U \mita{l0}]
)
)
)))

\end{array}\]

\begin{quote}\begin{verbatim}

@@
@@

-f-(-X-)-;
  >>> f(Z);

-...
g(Y);
h(Z);
\end{verbatim}\end{quote}

\[\begin{array}{l}
\mita{\sf{let}} \, \mita{\_aftret} = \msf{After} \vee \msf{Return} \, \mita{\sf{in}} \, \exists \mita{Z} . ((\exists \mita{X} . \exists \mita{v5} . \mita{-f-(-X-)-;
  \mth{>}\mth{>}\mth{>} f(Z);}_{\mita{v5}}) \wedge (\AX(\mita{\sf{let}} \, \mita{l0} = (\exists \mita{Y}\\\mbox{} . \mita{g(Y);}) \wedge (\AX(\mita{h(Z);})) \, \mita{\sf{in}} \, (\mita{\sf{let}} \, \mita{l1} = (\exists \mita{v2} . \mita{-\_S0}_{\mita{v2}}) \wedge (\neg ((\exists \mita{Y} . \mita{g(Y);}) \vee (\exists \mita{X} . \exists \mita{v3} . \mita{-f-(-X-)-;
  \mth{>}\mth{>}\mth{>} f(Z);}_{\mita{v3}})))\\\mbox{} \, \mita{\sf{in}} \, (\A[\mita{l1} \U (\mita{l0} \vee \mita{\_aftret})]
) \wedge (\E[\mita{l1} \U \mita{l0}]
)
)
)))

\end{array}\]

\begin{quote}\begin{verbatim}

@@
@@

-f-(-X-)-;
  >>> f(Z);

...
g(Y);
h(Z);
\end{verbatim}\end{quote}

\[\begin{array}{l}
\mita{\sf{let}} \, \mita{\_aftret} = \msf{After} \vee \msf{Return} \, \mita{\sf{in}} \, \exists \mita{Z} . ((\exists \mita{X} . \exists \mita{v4} . \mita{-f-(-X-)-;
  \mth{>}\mth{>}\mth{>} f(Z);}_{\mita{v4}}) \wedge (\AX(\mita{\sf{let}} \, \mita{l0} = (\exists \mita{Y}\\\mbox{} . \mita{g(Y);}) \wedge (\AX(\mita{h(Z);})) \, \mita{\sf{in}} \, (\mita{\sf{let}} \, \mita{l1} = \neg ((\exists \mita{Y} . \mita{g(Y);}) \vee (\exists \mita{X} . \exists \mita{v2} . \mita{-f-(-X-)-;
  \mth{>}\mth{>}\mth{>} f(Z);}_{\mita{v2}}))\\\mbox{} \, \mita{\sf{in}} \, (\A[\mita{l1} \U (\mita{l0} \vee \mita{\_aftret})]
) \wedge (\E[\mita{l1} \U \mita{l0}]
)
)
)))

\end{array}\]

\begin{quote}\begin{verbatim}

@@
@@

f(X);
...
g(Y);
h(Z);
\end{verbatim}\end{quote}

\[\begin{array}{l}
\mita{\sf{let}} \, \mita{\_aftret} = \msf{After} \vee \msf{Return} \, \mita{\sf{in}} \, (\exists \mita{X} . \mita{f(X);}) \wedge (\AX(\mita{\sf{let}} \, \mita{l0} = (\exists \mita{Y} . \mita{g(Y);}) \wedge (\AX(\exists \mita{Z}\\\mbox{} . \mita{h(Z);})) \, \mita{\sf{in}} \, (\mita{\sf{let}} \, \mita{l1} = \neg ((\exists \mita{Y} . \mita{g(Y);}) \vee (\exists \mita{X} . \mita{f(X);})) \, \mita{\sf{in}} \, (\A[\mita{l1} \U (\mita{l0} \vee \mita{\_aftret})]
)\\\mbox{} \wedge (\E[\mita{l1} \U \mita{l0}]
)
)
))

\end{array}\]

\begin{quote}\begin{verbatim}

@@
@@

f(X);
...   WHEN != h(Z)
g(Y);
h(Z);
\end{verbatim}\end{quote}

\[\begin{array}{l}
\mita{\sf{let}} \, \mita{\_aftret} = \msf{After} \vee \msf{Return} \, \mita{\sf{in}} \, (\exists \mita{X} . \mita{f(X);}) \wedge (\AX(\exists \mita{Z} . (\mita{\sf{let}} \, \mita{l0} = (\exists \mita{Y} . \mita{g(Y);}) \wedge (\AX(\mita{h(Z);}))\\\mbox{} \, \mita{\sf{in}} \, (\mita{\sf{let}} \, \mita{l1} = (\neg \mita{h(Z)}) \wedge (\neg ((\exists \mita{Y} . \mita{g(Y);}) \vee (\exists \mita{X} . \mita{f(X);}))) \, \mita{\sf{in}} \, (\A[\mita{l1} \U (\mita{l0} \vee \mita{\_aftret})]
)\\\mbox{} \wedge (\E[\mita{l1} \U \mita{l0}]
)
)
)))

\end{array}\]

\begin{quote}\begin{verbatim}

@@
@@

f(X);
...   WHEN != h(Q)
g(Y);
h(Z);
\end{verbatim}\end{quote}

\[\begin{array}{l}
\mita{\sf{let}} \, \mita{\_aftret} = \msf{After} \vee \msf{Return} \, \mita{\sf{in}} \, (\exists \mita{X} . \mita{f(X);}) \wedge (\AX(\mita{\sf{let}} \, \mita{l0} = (\exists \mita{Y} . \mita{g(Y);}) \wedge (\AX(\exists \mita{Z}\\\mbox{} . \mita{h(Z);})) \, \mita{\sf{in}} \, (\mita{\sf{let}} \, \mita{l1} = (\neg (\exists \mita{Q} . \mita{h(Q)})) \wedge (\neg ((\exists \mita{Y} . \mita{g(Y);}) \vee (\exists \mita{X} . \mita{f(X);}))) \, \mita{\sf{in}} \, (\A[\mita{l1}\\\mbox{} \U (\mita{l0} \vee \mita{\_aftret})]
) \wedge (\E[\mita{l1} \U \mita{l0}]
)
)
))

\end{array}\]

\begin{quote}\begin{verbatim}

@@
@@

if (X) {
  ...
} else {
  g(X);
}
h(Z);
\end{verbatim}\end{quote}

\[\begin{array}{l}
\mita{\sf{let}} \, \mita{\_aftret} = \msf{After} \vee \msf{Return} \, \mita{\sf{in}} \, \exists \mita{X} . (\mita{if (X) } \wedge (\AX((\msf{TrueBranch} \rightarrow (\AX(\exists \mita{v2} . (\mita{{\ttlb}
  }\\\mbox{} \wedge \msf{Paren}(v2) \wedge (\AX(\mita{\sf{let}} \, \mita{l0} = \mita{
{\ttrb}} \wedge \msf{Paren}(v2) \, \mita{\sf{in}} \, (\AF(\mita{l0} \vee \mita{\_aftret})) \wedge (\EF\mita{l0})
))))))\\\mbox{} \wedge (\msf{FalseBranch} \rightarrow (\AX(\exists \mita{v5} . (\mita{{\ttlb}
  } \wedge \msf{Paren}(v5) \wedge (\AX(\mita{g(X);} \wedge (\AX(\mita{
{\ttrb}} \wedge \msf{Paren}(v5)))))))))\\\mbox{} \wedge (\msf{After} \rightarrow (\AX(\exists \mita{Z} . \mita{h(Z);}))))) \wedge (\EX(\msf{FalseBranch})) \wedge (\EX(\msf{After})))

\end{array}\]

\begin{quote}\begin{verbatim}

@@
@@

<...
  
(
  h(X)
|
  g(Y)
)
...>
\end{verbatim}\end{quote}

\[\begin{array}{l}
\exists \mita{Y} . \exists \mita{X} . \AG(\mita{
(
h(X)
|
g(Y)
)} \vee (\neg \mita{
(
h(X)
|
g(Y)
)}))
\end{array}\]

\begin{quote}\begin{verbatim}

@@
@@

<...
  
(
  h(X)
|
  g(Y)
)
...>
r(X);
\end{verbatim}\end{quote}

\[\begin{array}{l}
\exists \mita{X} . \A[((\exists \mita{Y} . \mita{
(
h(X)
|
g(Y)
)}) \vee (\neg (\exists \mita{Y} . \mita{
(
h(X)
|
g(Y)
)}))) \U \mita{r(X);}]

\end{array}\]

\begin{quote}\begin{verbatim}

@@
@@


(
h(X)
|
g(Y)
)
\end{verbatim}\end{quote}

\[\begin{array}{l}
\exists \mita{Y} . \exists \mita{X} . \mita{
(
h(X)
|
g(Y)
)}
\end{array}\]

\begin{quote}\begin{verbatim}

@@
@@

m(Y);
?h(X);
g(Y);
\end{verbatim}\end{quote}

\[\begin{array}{l}
\exists \mita{Y} . (\mita{m(Y);} \wedge (\AX(\exists \mita{X} . ((\mita{h(X);} \wedge (\AX(\mita{g(Y);}))) \vee \mita{g(Y);}))))
\end{array}\]

\begin{quote}\begin{verbatim}

@@
@@

sht/*struct Scsi_Host_Template */.proc_info = proc_info_func;
\end{verbatim}\end{quote}

\[\begin{array}{l}
\exists \mita{proc\_info\_func} . \exists \mita{sht} . \mita{sht/*struct Scsi\_Host\_Template */.proc\_info = proc\_info\_func;}
\end{array}\]

\begin{quote}\begin{verbatim}

@@
@@

proc_info_func(char *buffer, char **start, off_t offset, int length,
               int hostno, int inout) {
  ...
  struct Scsi_Host *hostptr;
  ...
  hostptr = scsi_host_hn_get(hostno);
  ...
  ?if (hostptr == NULL) ?{
    ?...
  ?}
  ...
  ?scsi_host_put(hostptr);
  ...
}
\end{verbatim}\end{quote}

\[\begin{array}{l}
\mita{\sf{let}} \, \mita{\_aftret} = \msf{After} \vee \msf{Return} \, \mita{\sf{in}} \, \exists \mita{hostno} . ((\exists \mita{proc\_info\_func} . \exists \mita{buffer} . \exists \mita{start}\\\mbox{} . \exists \mita{offset} . \exists \mita{length} . \exists \mita{inout} . \mita{proc\_info\_func(char *buffer, char **start, off\_t offset, int length,
               int hostno, int inout) })\\\mbox{} \wedge (\AX(\exists \mita{v1} . (\mita{{\ttlb}
  } \wedge \msf{Paren}(v1) \wedge (\AX(\mita{\sf{let}} \, \mita{l21} = \exists \mita{hostptr} . (\mita{struct Scsi\_Host *hostptr;}\\\mbox{} \wedge (\AX(\mita{\sf{let}} \, \mita{l19} = \mita{hostptr = scsi\_host\_hn\_get(hostno);} \wedge (\AX(\mita{\sf{let}} \, \mita{l17} = (\mita{\sf{let}} \, \mita{l0} = \mita{
{\ttrb}}\\\mbox{} \wedge \msf{Paren}(v1) \, \mita{\sf{in}} \, (\mita{if (hostptr == NULL) } \wedge (\AX((\msf{TrueBranch} \vee \msf{After}) \wedge (\msf{TrueBranch}\\\mbox{} \rightarrow (\AX(\exists \mita{v21} . (\mita{{\ttlb}
  } \wedge \msf{Paren}(v21) \wedge (\AX(\mita{\sf{let}} \, \mita{l15} = \mita{
{\ttrb}} \wedge \msf{Paren}(v21) \, \mita{\sf{in}} \, (\AF(\mita{l15}\\\mbox{} \vee \mita{\_aftret})) \wedge (\EF\mita{l15})
)))))) \wedge (\msf{After} \rightarrow (\AX(\mita{\sf{let}} \, \mita{l13} = (\mita{scsi\_host\_put(hostptr);}\\\mbox{} \wedge (\AX(\mita{\sf{let}} \, \mita{l10} = \mita{l0} \, \mita{\sf{in}} \, (\mita{\sf{let}} \, \mita{l11} = \neg \mita{scsi\_host\_put(hostptr);} \, \mita{\sf{in}} \, (\A[\mita{l11} \U (\mita{l10}\\\mbox{} \vee \mita{\_aftret})]
) \wedge (\E[\mita{l11} \U \mita{l10}]
)
)
))) \vee (\mita{\sf{let}} \, \mita{l8} = \mita{l0} \, \mita{\sf{in}} \, (\mita{\sf{let}} \, \mita{l9} = \neg \mita{scsi\_host\_put(hostptr);}\\\mbox{} \, \mita{\sf{in}} \, (\A[\mita{l9} \U (\mita{l8} \vee \mita{\_aftret})]
) \wedge (\E[\mita{l9} \U \mita{l8}]
)
)
) \, \mita{\sf{in}} \, (\mita{\sf{let}} \, \mita{l14} = \neg (\mita{scsi\_host\_put(hostptr);}\\\mbox{} \vee (\mita{if (hostptr == NULL) } \wedge (\AX((\msf{TrueBranch} \vee \msf{After}) \wedge (\msf{TrueBranch} \rightarrow (\AX(\exists \mita{v16}\\\mbox{} . (\mita{{\ttlb}
  } \wedge \msf{Paren}(v16) \wedge (\AX(\mita{\sf{let}} \, \mita{l12} = \mita{
{\ttrb}} \wedge \msf{Paren}(v16) \, \mita{\sf{in}} \, (\AF(\mita{l12} \vee \mita{\_aftret}))\\\mbox{} \wedge (\EF\mita{l12})
)))))))))) \, \mita{\sf{in}} \, (\A[\mita{l14} \U (\mita{l13} \vee \mita{\_aftret})]
) \wedge (\E[\mita{l14} \U \mita{l13}]
)
)
)))))\\\mbox{} \wedge (\EX(\msf{After}))) \vee (\mita{\sf{let}} \, \mita{l6} = (\mita{scsi\_host\_put(hostptr);} \wedge (\AX(\mita{\sf{let}} \, \mita{l3} = \mita{l0} \, \mita{\sf{in}} \, (\mita{\sf{let}} \, \mita{l4} = \neg \mita{scsi\_host\_put(hostptr);}\\\mbox{} \, \mita{\sf{in}} \, (\A[\mita{l4} \U (\mita{l3} \vee \mita{\_aftret})]
) \wedge (\E[\mita{l4} \U \mita{l3}]
)
)
))) \vee (\mita{\sf{let}} \, \mita{l1} = \mita{l0} \, \mita{\sf{in}} \, (\mita{\sf{let}} \, \mita{l2} = \neg \mita{scsi\_host\_put(hostptr);}\\\mbox{} \, \mita{\sf{in}} \, (\A[\mita{l2} \U (\mita{l1} \vee \mita{\_aftret})]
) \wedge (\E[\mita{l2} \U \mita{l1}]
)
)
) \, \mita{\sf{in}} \, (\mita{\sf{let}} \, \mita{l7} = \neg ((\mita{if (hostptr == NULL) }\\\mbox{} \wedge (\AX((\msf{TrueBranch} \vee \msf{After}) \wedge (\msf{TrueBranch} \rightarrow (\AX(\exists \mita{v9} . (\mita{{\ttlb}
  } \wedge \msf{Paren}(v9) \wedge (\AX(\mita{\sf{let}} \, \mita{l5} = \mita{
{\ttrb}}\\\mbox{} \wedge \msf{Paren}(v9) \, \mita{\sf{in}} \, (\AF(\mita{l5} \vee \mita{\_aftret})) \wedge (\EF\mita{l5})
))))))))) \vee \mita{scsi\_host\_put(hostptr);})\\\mbox{} \, \mita{\sf{in}} \, (\A[\mita{l7} \U (\mita{l6} \vee \mita{\_aftret})]
) \wedge (\E[\mita{l7} \U \mita{l6}]
)
)
)
) \, \mita{\sf{in}} \, (\mita{\sf{let}} \, \mita{l18} = \neg ((\mita{if (hostptr == NULL) }\\\mbox{} \wedge (\AX((\msf{TrueBranch} \vee \msf{After}) \wedge (\msf{TrueBranch} \rightarrow (\AX(\exists \mita{v26} . (\mita{{\ttlb}
  } \wedge \msf{Paren}(v26) \wedge (\AX(\mita{\sf{let}} \, \mita{l16} = \mita{
{\ttrb}}\\\mbox{} \wedge \msf{Paren}(v26) \, \mita{\sf{in}} \, (\AF(\mita{l16} \vee \mita{\_aftret})) \wedge (\EF\mita{l16})
))))))))) \vee \mita{hostptr = scsi\_host\_hn\_get(hostno);})\\\mbox{} \, \mita{\sf{in}} \, (\A[\mita{l18} \U (\mita{l17} \vee \mita{\_aftret})]
) \wedge (\E[\mita{l18} \U \mita{l17}]
)
)
)) \, \mita{\sf{in}} \, (\mita{\sf{let}} \, \mita{l20} = \neg (\mita{hostptr = scsi\_host\_hn\_get(hostno);}\\\mbox{} \vee \mita{struct Scsi\_Host *hostptr;}) \, \mita{\sf{in}} \, (\A[\mita{l20} \U (\mita{l19} \vee \mita{\_aftret})]
) \wedge (\E[\mita{l20}\\\mbox{} \U \mita{l19}]
)
)
))) \, \mita{\sf{in}} \, (\mita{\sf{let}} \, \mita{l22} = \neg (\exists \mita{hostptr} . \mita{struct Scsi\_Host *hostptr;}) \, \mita{\sf{in}} \, (\A[\mita{l22}\\\mbox{} \U (\mita{l21} \vee \mita{\_aftret})]
) \wedge (\E[\mita{l22} \U \mita{l21}]
)
)
))))))

\end{array}\]

\begin{quote}\begin{verbatim}

@@
@@

proc_info_func(...) {
  <...
    
(
    E->host_no == hostno
|
    hostno
)
  ...>
}
\end{verbatim}\end{quote}

\[\begin{array}{l}
(\exists \mita{proc\_info\_func} . \mita{proc\_info\_func(...) }) \wedge (\AX(\exists \mita{v1} . (\mita{{\ttlb}
  } \wedge \msf{Paren}(v1) \wedge (\AX(\exists \mita{hostno}\\\mbox{} . \exists \mita{E} . \A[(\mita{
(
E-\mth{>}host\_no == hostno
|
hostno
)} \vee (\neg \mita{
(
E-\mth{>}host\_no == hostno
|
hostno
)}))\\\mbox{} \U (\mita{
{\ttrb}} \wedge \msf{Paren}(v1))]
)))))
\end{array}\]

\end{document}
